feat: sorted_concat

isabelle/Hoare/InsertionSort.thy
@@ -141,7 +141,90 @@ primrec head_swap_with where
 | "head_swap_with (x#xs) y = x#y#xs"
 
 fun removeAt where
-  "removeAt i xs = take (i-1) xs @ drop (i+1) xs"
+  "removeAt i xs = take i xs @ drop (i+1) xs"
+
+lemma removeAt_length: "i < length xs \<Longrightarrow> length (removeAt i xs) = length xs - 1"
+  apply (induct xs arbitrary: i)
+  apply auto
+  done
+
+lemma removeAt_at: "\<And>k. i < length xs \<Longrightarrow> removeAt i xs ! k = (if k < i then xs ! k else xs ! (k + 1))"
+  apply (induct xs arbitrary: i)
+  apply auto
+  apply (simp add: nth_append)
+  by (simp add: min.absorb2 nth_append)
+
+fun slice where
+  "slice i j xs = drop (i - 1) (take j xs)"
+
+lemma take_as_slice: "take n xs = slice 0 n xs"
+  by simp
+
+lemma sorted_for_slice: "sorted xs \<Longrightarrow> sorted (slice i j xs)"
+  by (simp add: sorted_drop sorted_take)
+
+lemma sorted_snoc:
+  assumes "sorted xs" "\<And>k. k < length xs \<Longrightarrow> xs ! k \<le> z"
+  shows "sorted (xs @ [z])"
+proof-
+  { fix n
+    have "n = length xs \<and> sorted xs \<and> (\<forall>k. k < length xs \<longrightarrow> xs ! k \<le> z) \<Longrightarrow> sorted (xs @ [z])"
+      apply (induct n arbitrary: xs)
+      apply auto
+    proof-
+      fix n xs
+      assume "(\<And>xs. n = length xs \<and> sorted xs \<and> (\<forall>k<length xs. xs ! k \<le> z) \<Longrightarrow> sorted (xs @ [z]))"
+        "Suc n = length xs" "sorted xs" "\<forall>k<length xs. xs ! k \<le> z"
+      obtain y ys where "xs = y # ys" "length ys = n"
+        by (meson Suc_length_conv \<open>Suc n = length xs\<close>)
+      have "sorted ys"
+        using \<open>sorted xs\<close> \<open>xs = y # ys\<close> sorted.simps(2) by blast
+      moreover have "\<forall>k < length ys. ys ! k \<le> z"
+        using \<open>\<forall>k<length xs. xs ! k \<le> z\<close> \<open>xs = y # ys\<close> by auto
+      ultimately have "sorted (ys @ [z])"
+        by (simp add: \<open>\<And>xs. n = length xs \<and> sorted xs \<and> (\<forall>k<length xs. xs ! k \<le> z) \<Longrightarrow> sorted (xs @ [z])\<close> \<open>length ys = n\<close>)
+
+      show "sorted (xs @ [z])"
+        using \<open>\<forall>k<length xs. xs ! k \<le> z\<close> \<open>sorted (ys @ [z])\<close> \<open>sorted xs\<close> \<open>xs = y # ys\<close> list.discI by auto
+    qed
+  }
+  hence "\<And>n. n = length xs \<and> sorted xs \<and> (\<forall>k. k < length xs \<longrightarrow> xs ! k \<le> z) \<Longrightarrow> sorted (xs @ [z])"
+    by simp
+
+  show ?thesis
+    by (simp add: \<open>\<And>n. n = length xs \<and> sorted xs \<and> (\<forall>k<length xs. xs ! k \<le> z) \<Longrightarrow> sorted (xs @ [z])\<close> assms(1) assms(2))
+qed
+
+lemma sorted_concat:
+  fixes xs :: "('a::linorder) list"
+  assumes "sorted xs" "sorted ys" "\<And>k. k < length xs \<Longrightarrow> xs ! k \<le> z" "\<And>k. k < length ys \<Longrightarrow> z \<le> ys ! k"
+  shows "sorted (xs @ [z] @ ys)"
+proof-
+  have "sorted (xs @ [z])"
+    by (simp add: assms(1) assms(3) sorted_snoc)
+  { fix n and xs :: "'a::linorder list" and ys :: "'a::linorder list"
+    have "length ys = n \<Longrightarrow> sorted xs \<Longrightarrow> sorted ys \<Longrightarrow> (\<And>k. ys \<noteq> [] \<Longrightarrow> k < length xs \<Longrightarrow> xs ! k \<le> ys ! 0) \<Longrightarrow> sorted (xs @ ys)"
+      apply (induct n arbitrary: xs ys)
+      apply simp
+    proof-
+      fix n and xs :: "'a::linorder list" and ys :: "'a::linorder list"
+      assume hyp: "(\<And>(xs :: 'a::linorder list) ys. length ys = n \<Longrightarrow> sorted xs \<Longrightarrow> sorted ys \<Longrightarrow> (\<And>k. ys \<noteq> [] \<Longrightarrow> k < length xs \<Longrightarrow> xs ! k \<le> ys ! 0) \<Longrightarrow> sorted (xs @ ys))"
+        and "length ys = Suc n" "sorted xs" "sorted ys" "(\<And>k. ys \<noteq> [] \<Longrightarrow> k < length xs \<Longrightarrow> xs ! k \<le> ys ! 0)"
+      obtain w and ws :: "'a::linorder list" where "ys = w # ws" "length ws = n"
+        by (metis Suc_length_conv \<open>length ys = Suc n\<close>)
+      have "sorted ws"
+        using \<open>sorted ys\<close> \<open>ys = w # ws\<close> sorted.simps(2) by blast
+      moreover have "sorted (xs @ [w])"
+        using \<open>\<And>k. \<lbrakk>ys \<noteq> []; k < length xs\<rbrakk> \<Longrightarrow> xs ! k \<le> ys ! 0\<close> \<open>sorted xs\<close> \<open>ys = w # ws\<close> sorted_snoc by auto
+      moreover have "\<And>k. ws \<noteq> [] \<Longrightarrow> k < length (xs @ [w]) \<Longrightarrow> (xs @ [w]) ! k \<le> ws ! 0"
+        by (metis (no_types, hide_lams) \<open>\<And>k. \<lbrakk>ys \<noteq> []; k < length xs\<rbrakk> \<Longrightarrow> xs ! k \<le> ys ! 0\<close> \<open>sorted ys\<close> \<open>ys = w # ws\<close> dual_order.trans length_append_singleton less_Suc_eq list.distinct(1) list.exhaust nth_Cons_0 nth_append nth_append_length sorted2)
+      ultimately show "sorted (xs @ ys)"
+        using \<open>length ws = n\<close> \<open>ys = w # ws\<close> hyp by fastforce
+    qed
+  }
+  thus ?thesis
+    by (metis append_Cons append_Nil assms(1) assms(2) assms(3) assms(4) length_greater_0_conv nth_Cons_0 sorted.elims(2) sorted1 sorted2)
+qed
 
 lemma "
   VARS H i j tmp
@@ -166,22 +249,136 @@ proof-
   show "\<And>H i j tmp. array H arr N xs \<Longrightarrow> \<exists>zs. array H arr (1 - 1) zs \<and> sorted zs"
     apply simp
     using array.intros(1) sorted.simps(1) by blast
-  show "\<And>H i j tmp. (\<exists>zs. array H arr (i - 1) zs \<and> sorted zs) \<and> i < N \<Longrightarrow> \<exists>zs'. i \<le> i \<and> array H arr (i - 1) zs' \<and> sorted (removeAt i zs')"
+  show "\<And>H i j tmp. (\<exists>zs. array H arr (i - 1) zs \<and> sorted zs) \<and> i < N \<Longrightarrow> (\<exists>zs'. i \<le> i \<and> array H arr (i - 1) zs' \<and> sorted (removeAt i zs'))"
     sorry
 
   show "\<And>H i j tmp.
-       (\<exists>zs'. j \<le> i \<and> array H arr (i - 1) zs' \<and> sorted (removeAt j zs')) \<and> 0 < j \<and> the (H (arr + j)) < the (H (arr + j - 1)) \<Longrightarrow>
-       \<exists>zs'. j - 1 \<le> i \<and> array (H(arr + j \<mapsto> the (H (arr + j - 1)), arr + j - 1 \<mapsto> the (H (arr + j)))) arr (i - 1) zs' \<and> sorted (removeAt (j - 1) zs')"
+       ((\<exists>zs'. j \<le> i \<and> array H arr (i - 1) zs' \<and> sorted (removeAt j zs'))) \<and> 0 < j \<and> the (H (arr + j)) < the (H (arr + j - 1)) \<Longrightarrow>
+       (\<exists>zs'. j - 1 \<le> i \<and> array (H(arr + j \<mapsto> the (H (arr + j - 1)), arr + j - 1 \<mapsto> the (H (arr + j)))) arr (i - 1) zs' \<and> sorted (removeAt (j - 1) zs'))"
   proof-
     fix H i j tmp
-    assume "(\<exists>zs'. j \<le> i \<and> array H arr (i - 1) zs' \<and> sorted (removeAt j zs')) \<and> 0 < j \<and> the (H (arr + j)) < the (H (arr + j - 1))"
-    obtain zs' where "j \<le> i \<and> array H arr (i - 1) zs' \<and> sorted (removeAt j zs')"
-      using \<open>(\<exists>zs'. j \<le> i \<and> array H arr (i - 1) zs' \<and> sorted (removeAt j zs')) \<and> 0 < j \<and> the (H (arr + j)) < the (H (arr + j - 1))\<close> by blast
-    have "j - 1 \<le> i"
-      using \<open>j \<le> i \<and> array H arr (i - 1) zs' \<and> sorted (removeAt j zs')\<close> le_diff_conv trans_le_add1 by blast
-    define zs where "zs \<equiv> swapAt j (j - 1) zs'"
-    have "array (H(arr + j \<mapsto> the (H (arr + j - 1)), arr + j - 1 \<mapsto> the (H (arr + j)))) arr (i - 1) zs"
-      apply (simp add: zs_def)
+    assume "((\<exists>zs'. j \<le> i \<and> array H arr (i - 1) zs' \<and> sorted (removeAt j zs'))) \<and> 0 < j \<and> the (H (arr + j)) < the (H (arr + j - 1))"
+    obtain xs where "j \<le> i \<and> array H arr (i - 1) xs \<and> sorted (removeAt j xs)"
+      using \<open>((\<exists>zs'. j \<le> i \<and> array H arr (i - 1) zs' \<and> sorted (removeAt j zs'))) \<and> 0 < j \<and> the (H (arr + j)) < the (H (arr + j - 1))\<close> by blast
+
+    obtain ys where "array (H(arr + j \<mapsto> the (H (arr + j - 1)))) arr (i - 1) ys" "\<And>k. k < length ys \<Longrightarrow> ys ! k = (if arr + k = arr + j then the (H (arr + j - 1)) else xs ! k)"
+      apply (rule array_exists_under_heap_modification [of "H" arr "i - 1" xs "arr + j" "the (H (arr + j - 1))"])
+      using \<open>j \<le> i \<and> array H arr (i - 1) xs \<and> sorted (removeAt j xs)\<close> apply blast
+      by (simp add: array_length)
+    obtain zs where "array (H(arr + j \<mapsto> the (H (arr + j - 1)), arr + j - 1 \<mapsto> the (H (arr + j)))) arr (i - 1) zs" "\<And>k. k < length zs \<Longrightarrow> zs ! k = (if arr + k = arr + j - 1 then the (H (arr + j)) else ys ! k)"
+      apply (rule array_exists_under_heap_modification [of "H(arr + j \<mapsto> the (H (arr + j - 1)))" arr "i - 1" ys "arr + j - 1" "the (H (arr + j))"])
+      using \<open>array (H(arr + j \<mapsto> the (H (arr + j - 1)))) arr (i - 1) ys\<close> apply blast
+      by (simp add: array_length)
+
+    have "length zs = i - 1"
+      using \<open>array (H(arr + j \<mapsto> the (H (arr + j - 1)), arr + j - 1 \<mapsto> the (H (arr + j)))) arr (i - 1) zs\<close> array_length by blast
+    have "length ys = i - 1"
+      using \<open>array (H(arr + j \<mapsto> the (H (arr + j - 1)))) arr (i - 1) ys\<close> array_length by blast
+
+    have "\<And>k. k < length zs \<Longrightarrow> zs ! k = (if k = j - 1 then the (H (arr + j)) else if k = j then the (H (arr + j - 1)) else xs ! k)"
+      by (metis (no_types, lifting) Nat.add_diff_assoc One_nat_def Suc_leI \<open>(\<exists>zs'. j \<le> i \<and> array H arr (i - 1) zs' \<and> sorted (removeAt j zs')) \<and> 0 < j \<and> the (H (arr + j)) < the (H (arr + j - 1))\<close> \<open>\<And>k. k < length ys \<Longrightarrow> ys ! k = (if arr + k = arr + j then the (H (arr + j - 1)) else xs ! k)\<close> \<open>\<And>k. k < length zs \<Longrightarrow> zs ! k = (if arr + k = arr + j - 1 then the (H (arr + j)) else ys ! k)\<close> \<open>length ys = i - 1\<close> \<open>length zs = i - 1\<close> add_diff_cancel_left')
+
+    have "sorted (removeAt j xs)"
+      using \<open>j \<le> i \<and> array H arr (i - 1) xs \<and> sorted (removeAt j xs)\<close> by blast
+
+    { assume "j = i"
+      have "\<And>k. k < i - 1 \<Longrightarrow> zs ! k = xs ! k"
+        by (simp add: \<open>\<And>k. k < length zs \<Longrightarrow> zs ! k = (if k = j - 1 then the (H (arr + j)) else if k = j then the (H (arr + j - 1)) else xs ! k)\<close> \<open>j = i\<close> \<open>length zs = i - 1\<close> less_not_refl3)
+      have "removeAt (i - 1) zs = removeAt (i - 1) xs"
+        by (metis \<open>\<And>k. k < i - 1 \<Longrightarrow> zs ! k = xs ! k\<close> \<open>j \<le> i \<and> array H arr (i - 1) xs \<and> sorted (removeAt j xs)\<close> \<open>length zs = i - 1\<close> array_length nth_equalityI)
+      have "sorted (removeAt (i - 1) zs)"
+        by (metis One_nat_def Suc_pred \<open>(\<exists>zs'. j \<le> i \<and> array H arr (i - 1) zs' \<and> sorted (removeAt j zs')) \<and> 0 < j \<and> the (H (arr + j)) < the (H (arr + j - 1))\<close> \<open>j = i\<close> \<open>j \<le> i \<and> array H arr (i - 1) xs \<and> sorted (removeAt j xs)\<close> \<open>removeAt (i - 1) zs = removeAt (i - 1) xs\<close> add.commute append_Nil2 array_length diff_le_self drop_all order_refl plus_1_eq_Suc removeAt.simps sorted_append take_all)
+      have "sorted (removeAt (j - 1) zs)"
+        using \<open>j = i\<close> \<open>sorted (removeAt (i - 1) zs)\<close> by blast
+    }
+    hence "j = i \<Longrightarrow> sorted (removeAt (j - 1) zs)"
+      by blast
+
+    { assume "j = i - 1"
+      have "j - 1 < length zs"
+        using \<open>(\<exists>zs'. j \<le> i \<and> array H arr (i - 1) zs' \<and> sorted (removeAt j zs')) \<and> 0 < j \<and> the (H (arr + j)) < the (H (arr + j - 1))\<close> \<open>j = i - 1\<close> \<open>length zs = i - 1\<close> by linarith
+      have "\<And>k. k < j - 1 \<Longrightarrow> zs ! k = xs ! k"
+        using \<open>\<And>k. k < length zs \<Longrightarrow> zs ! k = (if k = j - 1 then the (H (arr + j)) else if k = j then the (H (arr + j - 1)) else xs ! k)\<close> \<open>j = i - 1\<close> \<open>length zs = i - 1\<close> by auto
+      have "length zs = j"
+        by (simp add: \<open>j = i - 1\<close> \<open>length zs = i - 1\<close>)
+      have "length (removeAt (j - 1) zs) = j - 1"
+        using \<open>j - 1 < length zs\<close> \<open>length zs = j\<close> removeAt_length by blast
+      have "\<And>k. k < length (removeAt (j - 1) zs) \<Longrightarrow> removeAt (j - 1) zs ! k = removeAt (j - 1) xs ! k"
+        by (metis \<open>\<And>k. k < j - 1 \<Longrightarrow> zs ! k = xs ! k\<close> \<open>j - 1 < length zs\<close> \<open>j = i - 1\<close> \<open>j \<le> i \<and> array H arr (i - 1) xs \<and> sorted (removeAt j xs)\<close> \<open>length (removeAt (j - 1) zs) = j - 1\<close> \<open>length zs = j\<close> array_length removeAt_at)
+
+      have "removeAt (j - 1) zs = removeAt (j - 1) xs"
+        by (metis \<open>\<And>k. k < length (removeAt (j - 1) zs) \<Longrightarrow> removeAt (j - 1) zs ! k = removeAt (j - 1) xs ! k\<close> \<open>j - 1 < length zs\<close> \<open>j = i - 1\<close> \<open>j \<le> i \<and> array H arr (i - 1) xs \<and> sorted (removeAt j xs)\<close> \<open>length zs = j\<close> array_length nth_equalityI removeAt_length)
+      have "sorted (removeAt (j - 1) zs)"
+        by (metis One_nat_def Suc_pred \<open>(\<exists>zs'. j \<le> i \<and> array H arr (i - 1) zs' \<and> sorted (removeAt j zs')) \<and> 0 < j \<and> the (H (arr + j)) < the (H (arr + j - 1))\<close> \<open>j = i - 1\<close> \<open>j \<le> i \<and> array H arr (i - 1) xs \<and> sorted (removeAt j xs)\<close> \<open>removeAt (j - 1) zs = removeAt (j - 1) xs\<close> add.commute append_Nil2 array_length drop_all order_refl plus_1_eq_Suc removeAt.simps sorted_append sorted_take take_all)
+    }
+    hence "j = i - 1 \<Longrightarrow> sorted (removeAt (j - 1) zs)"
+      by blast
+
+    { assume "j < i - 1"
+      have "j < length zs"
+        using \<open>j < i - 1\<close> \<open>length zs = i - 1\<close> by auto
+      have "\<And>k. k < j - 1 \<Longrightarrow> zs ! k = xs ! k"
+        using \<open>\<And>k. k < length zs \<Longrightarrow> zs ! k = (if k = j - 1 then the (H (arr + j)) else if k = j then the (H (arr + j - 1)) else xs ! k)\<close> \<open>j < i - 1\<close> \<open>length zs = i - 1\<close> by auto
+      have "zs ! (j - 1) = the (H (arr + j))"
+        by (simp add: \<open>\<And>k. k < length zs \<Longrightarrow> zs ! k = (if k = j - 1 then the (H (arr + j)) else if k = j then the (H (arr + j - 1)) else xs ! k)\<close> \<open>j < length zs\<close> less_imp_diff_less)
+      have "zs ! j = the (H (arr + j - 1))"
+        using \<open>(\<exists>zs'. j \<le> i \<and> array H arr (i - 1) zs' \<and> sorted (removeAt j zs')) \<and> 0 < j \<and> the (H (arr + j)) < the (H (arr + j - 1))\<close> \<open>\<And>k. k < length zs \<Longrightarrow> zs ! k = (if k = j - 1 then the (H (arr + j)) else if k = j then the (H (arr + j - 1)) else xs ! k)\<close> \<open>j < length zs\<close> by auto
+
+      have "xs ! (j - 1) = the (H (arr + j - 1))"
+        by (metis (mono_tags, lifting) Nat.add_diff_assoc One_nat_def Suc_leI \<open>(\<exists>zs'. j \<le> i \<and> array H arr (i - 1) zs' \<and> sorted (removeAt j zs')) \<and> 0 < j \<and> the (H (arr + j)) < the (H (arr + j - 1))\<close> \<open>j < length zs\<close> \<open>j \<le> i \<and> array H arr (i - 1) xs \<and> sorted (removeAt j xs)\<close> \<open>length zs = i - 1\<close> array_list_at less_imp_diff_less option.sel)
+      have "\<And>k. k < j - 1 \<Longrightarrow> (removeAt j xs) ! k \<le> (removeAt j xs) ! (j - 1)"
+        by (metis One_nat_def Suc_leI \<open>(\<exists>zs'. j \<le> i \<and> array H arr (i - 1) zs' \<and> sorted (removeAt j zs')) \<and> 0 < j \<and> the (H (arr + j)) < the (H (arr + j - 1))\<close> \<open>j < i - 1\<close> \<open>j \<le> i \<and> array H arr (i - 1) xs \<and> sorted (removeAt j xs)\<close> array_length diff_less_mono less_imp_le_nat removeAt_length sorted_nth_mono)
+      have "\<And>k. k < j - 1 \<Longrightarrow> (removeAt j xs) ! k = xs ! k \<and> (removeAt j xs) ! (j - 1) = xs ! (j - 1)"
+        by (metis One_nat_def Suc_pred \<open>(\<exists>zs'. j \<le> i \<and> array H arr (i - 1) zs' \<and> sorted (removeAt j zs')) \<and> 0 < j \<and> the (H (arr + j)) < the (H (arr + j - 1))\<close> \<open>j < i - 1\<close> \<open>j \<le> i \<and> array H arr (i - 1) xs \<and> sorted (removeAt j xs)\<close> array_length less_Suc_eq removeAt_at)
+      have "\<And>k. k < j - 1 \<Longrightarrow> xs ! k \<le> xs ! (j - 1)"
+        using \<open>\<And>k. k < j - 1 \<Longrightarrow> removeAt j xs ! k = xs ! k \<and> removeAt j xs ! (j - 1) = xs ! (j - 1)\<close> \<open>\<And>k. k < j - 1 \<Longrightarrow> removeAt j xs ! k \<le> removeAt j xs ! (j - 1)\<close> by auto
+      have "\<And>k. k < j - 1 \<Longrightarrow> zs ! k \<le> zs ! j"
+        using \<open>\<And>k. k < j - 1 \<Longrightarrow> xs ! k \<le> xs ! (j - 1)\<close> \<open>\<And>k. k < j - 1 \<Longrightarrow> zs ! k = xs ! k\<close> \<open>xs ! (j - 1) = the (H (arr + j - 1))\<close> \<open>zs ! j = the (H (arr + j - 1))\<close> by auto
+
+      have "\<And>k. j < k \<and> k < length zs \<Longrightarrow> zs ! k = xs ! k"
+        using \<open>\<And>k. k < length zs \<Longrightarrow> zs ! k = (if k = j - 1 then the (H (arr + j)) else if k = j then the (H (arr + j - 1)) else xs ! k)\<close> by auto
+      have "\<And>k. j < k \<and> k < length zs \<Longrightarrow> zs ! j \<le> zs ! k"
+      proof-
+        fix k 
+        assume "j < k \<and> k < length zs"
+        have "zs ! j = the (H (arr + j - 1))"
+          using \<open>zs ! j = the (H (arr + j - 1))\<close> by blast
+        have "zs ! k = xs ! k"
+          using \<open>\<And>k. j < k \<and> k < length zs \<Longrightarrow> zs ! k = xs ! k\<close> \<open>j < k \<and> k < length zs\<close> by blast
+        also have "xs ! k = (removeAt j xs) ! (k - 1)"
+          by (smt One_nat_def Suc_leI Suc_pred \<open>(\<exists>zs'. j \<le> i \<and> array H arr (i - 1) zs' \<and> sorted (removeAt j zs')) \<and> 0 < j \<and> the (H (arr + j)) < the (H (arr + j - 1))\<close> \<open>j < i - 1\<close> \<open>j < k \<and> k < length zs\<close> \<open>j \<le> i \<and> array H arr (i - 1) xs \<and> sorted (removeAt j xs)\<close> array_length leD le_add_diff_inverse2 less_trans removeAt_at)
+        finally have "zs ! k = (removeAt j xs) ! (k - 1)"
+          by simp
+
+        have "\<And>k. j \<le> k \<and> k < length (removeAt j xs) \<Longrightarrow> (removeAt j xs) ! (j - 1) \<le> (removeAt j xs) ! k"
+          by (metis \<open>j \<le> i \<and> array H arr (i - 1) xs \<and> sorted (removeAt j xs)\<close> diff_le_self less_imp_diff_less nat_less_le sorted_nth_mono)
+        have "removeAt j xs ! (j - 1) = the (H (arr + j - 1))"
+          by (metis One_nat_def \<open>(\<exists>zs'. j \<le> i \<and> array H arr (i - 1) zs' \<and> sorted (removeAt j zs')) \<and> 0 < j \<and> the (H (arr + j)) < the (H (arr + j - 1))\<close> \<open>j < i - 1\<close> \<open>j \<le> i \<and> array H arr (i - 1) xs \<and> sorted (removeAt j xs)\<close> \<open>xs ! (j - 1) = the (H (arr + j - 1))\<close> array_length diff_Suc_less removeAt_at)
+
+        show "zs ! j \<le> zs ! k"
+          by (metis (no_types, lifting) One_nat_def Suc_leI Suc_pred \<open>(\<exists>zs'. j \<le> i \<and> array H arr (i - 1) zs' \<and> sorted (removeAt j zs')) \<and> 0 < j \<and> the (H (arr + j)) < the (H (arr + j - 1))\<close> \<open>\<And>k. j \<le> k \<and> k < length (removeAt j xs) \<Longrightarrow> removeAt j xs ! (j - 1) \<le> removeAt j xs ! k\<close> \<open>j < k \<and> k < length zs\<close> \<open>j \<le> i \<and> array H arr (i - 1) xs \<and> sorted (removeAt j xs)\<close> \<open>length zs = i - 1\<close> \<open>removeAt j xs ! (j - 1) = the (H (arr + j - 1))\<close> \<open>zs ! j = the (H (arr + j - 1))\<close> \<open>zs ! k = removeAt j xs ! (k - 1)\<close> array_length diff_less_mono less_trans removeAt_length)
+      qed
+
+      have "sorted (removeAt (j - 1) zs)"
+      proof-
+        { fix k
+          assume "k < length (removeAt (j - 1) zs)"
+
+          have "k < j - 1 \<Longrightarrow> (removeAt (j - 1) zs) ! k \<le> (removeAt (j - 1) zs) ! (j - 1)"
+            by (metis One_nat_def Suc_leI \<open>(\<exists>zs'. j \<le> i \<and> array H arr (i - 1) zs' \<and> sorted (removeAt j zs')) \<and> 0 < j \<and> the (H (arr + j)) < the (H (arr + j - 1))\<close> \<open>\<And>k. k < j - 1 \<Longrightarrow> zs ! k \<le> zs ! j\<close> \<open>j < i - 1\<close> \<open>length zs = i - 1\<close> le_add_diff_inverse2 less_imp_diff_less neq_iff removeAt_at)
+          have "j \<le> k \<Longrightarrow> (removeAt (j - 1) zs) ! (j - 1) \<le> (removeAt (j - 1) zs) ! k"
+            by (smt One_nat_def Suc_less_eq \<open>(\<exists>zs'. j \<le> i \<and> array H arr (i - 1) zs' \<and> sorted (removeAt j zs')) \<and> 0 < j \<and> the (H (arr + j)) < the (H (arr + j - 1))\<close> \<open>\<And>k. j < k \<and> k < length zs \<Longrightarrow> zs ! j \<le> zs ! k\<close> \<open>j < i - 1\<close> \<open>k < length (removeAt (j - 1) zs)\<close> \<open>length zs = i - 1\<close> add.commute leD le_add_diff_inverse2 less_Suc_eq less_Suc_eq_le less_trans plus_1_eq_Suc removeAt_at removeAt_length)
+
+          have "sorted (take (j - 2) (removeAt (j - 1) zs))"
+          proof-
+            have "take (j - 2) (removeAt (j - 1) zs) = take (j - 2) (removeAt j xs)"
+
+        }
+    }
+
+    have "sorted (removeAt (j - 1) zs)"
+    proof-
+      have "zs ! (j - 1) = xs ! j"
 
     show "\<exists>zs'. j - 1 \<le> i \<and> array (H(arr + j \<mapsto> the (H (arr + j - 1)), arr + j - 1 \<mapsto> the (H (arr + j)))) arr (i - 1) zs' \<and> sorted (removeAt (j - 1) zs')"
 
